src/CodeStorage.v
@@ -31,9 +31,9 @@ Section Defs.
 
   Definition is_fresh cm vh := negb (contains _ VersionedHash.eq_dec (cm_fresh cm) vh).
 
-  Inductive code_fetch_no_masking: depot -> code_storage
+  Inductive code_fetch_no_masking: shard -> code_storage
                         -> contract_address -> (versioned_hash * code_page * code_length) -> Prop :=
-  | cfnm_load : forall (contracts:depot) (called_address:contract_address) deployer_storage hash_enc (code_storage:code_storage) code_length_in_words extra_marker partial_hash page_init,
+  | cfnm_load : forall (contracts:shard) (called_address:contract_address) deployer_storage hash_enc (code_storage:code_storage) code_length_in_words extra_marker partial_hash page_init,
       load_result _ DEPLOYER_SYSTEM_CONTRACT_ADDRESS contracts deployer_storage ->
       load_result storage_params (@resize _ 256 called_address) deployer_storage hash_enc ->
       hash_enc <> zero256 ->
@@ -42,14 +42,22 @@ Section Defs.
       load_result (code_storage_params) (@resize _ 256 partial_hash) code_storage page_init ->
       code_fetch_no_masking contracts code_storage called_address ((mk_vhash code_length_in_words extra_marker partial_hash), page_init,code_length_in_words).
 
-  Inductive code_fetch: bool -> depot -> code_storage -> contract_address -> (versioned_hash * code_page * code_length) -> Prop :=
-  | cfh_load is_masking_allowed: forall (contracts:depot) (called_address:contract_address) (code_storage:code_storage) code_length_in_words extra_marker partial_hash page_init,
+  Inductive code_fetch_shard: bool -> shard -> code_storage -> contract_address -> (versioned_hash * code_page * code_length) -> Prop :=
+  | cfh_load is_masking_allowed: forall (contracts:shard) (called_address:contract_address) (code_storage:code_storage) code_length_in_words extra_marker partial_hash page_init,
       code_fetch_no_masking contracts code_storage called_address ((mk_vhash code_length_in_words extra_marker partial_hash), page_init,code_length_in_words) ->
-      code_fetch is_masking_allowed contracts code_storage called_address ((mk_vhash code_length_in_words extra_marker partial_hash), page_init,code_length_in_words)
+      code_fetch_shard is_masking_allowed contracts code_storage called_address ((mk_vhash code_length_in_words extra_marker partial_hash), page_init,code_length_in_words)
 
-  | cfh_load_aa_default : forall (contracts:depot) (called_address:contract_address) deployer_storage (code_storage:code_storage),
+  | cfh_load_aa_default : forall (contracts:shard) (called_address:contract_address) deployer_storage (code_storage:code_storage),
       load_result _ DEPLOYER_SYSTEM_CONTRACT_ADDRESS contracts deployer_storage ->
       load_result storage_params (@resize _ 256 called_address) deployer_storage zero256->
-      code_fetch true contracts code_storage called_address (DEFAULT_AA_VHASH, DEFAULT_AA_CODE _ invalid_ins,code_length_in_words DEFAULT_AA_VHASH).
+      code_fetch_shard true contracts code_storage called_address (DEFAULT_AA_VHASH, DEFAULT_AA_CODE _ invalid_ins,code_length_in_words DEFAULT_AA_VHASH).
 
+  Inductive code_fetch (depot:depot) (sid: shard_id): bool -> code_storage -> contract_address ->
+                                                      (versioned_hash * code_page * code_length) -> Prop :=
+| cfs_fetch: forall masking_allowed sh codes addr vh,
+    load_result _ sid depot sh ->
+    code_fetch_shard masking_allowed sh codes addr vh ->
+    code_fetch depot sid masking_allowed codes addr vh .
+  
+    
 End Defs.
