src/sem/Farcall.v
@@ -2,28 +2,28 @@ From RecordUpdate Require Import RecordSet.
 Require Common Ergs Condition CallStack Memory Instruction State MemoryOps ABI SemanticCommon.
 
 Import
-BinIntDef.Z
-Bool
-List
-ListNotations
-ZArith
-ZMod.
+  BinIntDef.Z
+    Bool
+    List
+    ListNotations
+    ZArith
+    ZMod.
 
 
 Import
-Addressing
-ABI ABI.FarCall ABI.FatPointer
-CodeStorage
-Common
-Condition
-Ergs
-CallStack
-Memory
-MemoryBase
-MemoryOps
-RecordSetNotations
-SemanticCommon
-State.
+  Addressing
+    ABI ABI.FarCall ABI.FatPointer
+    CodeStorage
+    Common
+    Condition
+    Ergs
+    CallStack
+    Memory
+    MemoryBase
+    MemoryOps
+    RecordSetNotations
+    SemanticCommon
+    State.
 
 Import Instruction Addressing.Coercions.
 
@@ -51,11 +51,11 @@ VM state is described through the following main predicates:
 - [farcall]
 
 If you know about fetching operands for instructions and the instruction fetching described in [Semantics.step], start investigating farcalls from the [farcall] predicate.
-*)
+ *)
 Section Parameters.
-Open Scope Z.
+  Open Scope Z.
 
-(**
+  (**
 
 ## Global farcall parameters
 
@@ -67,17 +67,17 @@ Open Scope Z.
 
    Therefore, addresses in range from 0 inclusive to [INITIAL_SP_ON_FAR_CALL]
    exclusive can be used as a scratch space.
-*)
+   *)
 
-Definition INITIAL_SP_ON_FAR_CALL : stack_address := 1024.
+  Definition INITIAL_SP_ON_FAR_CALL : stack_address := 1024.
 
-(**
+  (**
 2. Initial heap and auxheap pages bound.
 
    The heap and auxheap pages start with [NEW_FRAME_MEMORY_STIPEND] bound.
    Growing them beyond this bound costs ergs.
-*)
-Definition NEW_FRAME_MEMORY_STIPEND : mem_address := 1024.
+   *)
+  Definition NEW_FRAME_MEMORY_STIPEND : mem_address := 1024.
 
 End Parameters.
 
@@ -85,7 +85,7 @@ End Parameters.
 3. Maximal fraction of ergs allowed to pass.
 
    It is not allowed to pass more than 63/64th of your remaining ergs to a far call.
-*)
+ *)
 Definition max_passable (remaining:ergs) : ergs := (((int_val _ remaining) / 64 ) * 63)%Z.
 Inductive pass_allowed_ergs : (ergs * callstack )-> ergs * callstack -> Prop :=
 | pae_apply: forall xstack1 xstack2 pass_ergs_query,
@@ -112,7 +112,7 @@ Far call creates a new execution context with new pages for:
 - auxheap
 
 The initial bounds for the new heap and auxheap pages are set to [NEW_FRAME_MEMORY_STIPEND].
-*)
+ *)
 Inductive alloc_pages_extframe:  (pages * active_pages) -> code_page -> pages * active_pages -> Prop :=
 | ape_alloc: forall code mm ctx code_id const_id stack_id heap_id heap_aux_id,
     code_id = length mm ->
@@ -153,16 +153,16 @@ Inductive decommitment_cost (cm:code_manager) vhash (code_length_in_words: code_
 (** Fetch code and pay the associated cost. If [masking_allowed] is true and there is no code
 associated with a given contract address, then the default AA code will be
 fetched. See [code_fetch]. *)
-Inductive paid_code_fetch masking_allowed: depot -> code_manager -> contract_address
-                               -> callstack -> callstack * code_page
-                               ->Prop :=
+Inductive paid_code_fetch masking_allowed sid: depot -> code_manager -> contract_address
+                                           -> callstack -> callstack * code_page
+                                           ->Prop :=
 | cfp_apply:
   forall depot codes (dest_addr: contract_address) vhash dest_addr new_code_page code_length cost__decomm xstack0 xstack1,
 
-    code_fetch _ _ masking_allowed depot codes.(cm_storage _ _) dest_addr (vhash, new_code_page, code_length) ->
+    code_fetch _ _ depot sid masking_allowed codes.(cm_storage _ _) dest_addr (vhash, new_code_page, code_length) ->
     decommitment_cost codes vhash code_length cost__decomm ->
     pay cost__decomm xstack0 xstack1 ->
-    paid_code_fetch masking_allowed depot codes dest_addr xstack0 (xstack1, new_code_page).
+    paid_code_fetch masking_allowed sid depot codes dest_addr xstack0 (xstack1, new_code_page).
 
 (** ## System calls
 
@@ -170,7 +170,7 @@ A system call is a far call that satisfies the following conditions:
 
 - The destination is a kernel address.
 - The field `is_system` of [FarCall.params] passed through an operand is set to 1.
-*)
+ *)
 
 
 (** # Far call instructions
@@ -312,7 +312,7 @@ Record versioned_hash := {
     + Registers `r3`, `r4`, ..., `r15` are reserved; their pointer tags are
       cleared, but their values are unchanged.
     + Registers `r14` and `r15` are cleared.
-*)
+ *)
 Definition regs_effect regs (is_system is_ctor:bool) ptr :=
   let far_call_r2 :=
     let is_system_bit := Z.shiftl is_system 1 in
@@ -320,27 +320,27 @@ Definition regs_effect regs (is_system is_ctor:bool) ptr :=
     let bits := Z.lor is_system_bit is_ctor_bit in
     IntValue (int_mod_of word_bits bits) in
   let enc_ptr := FatPointer.ABI.(encode) ptr in
-     if is_system then
-       regs
-       <| gprs_r1 := PtrValue enc_ptr |>
-       <| gprs_r2 := far_call_r2      |>
-       (* In system calls, preserve values in r3-r13 but clear ptr tags *)
-       <| gprs_r3 ::= clear_pointer_tag |>
-       <| gprs_r4 ::= clear_pointer_tag |>
-       <| gprs_r5 ::= clear_pointer_tag |>
-       <| gprs_r6 ::= clear_pointer_tag |>
-       <| gprs_r7 ::= clear_pointer_tag |>
-       <| gprs_r8 ::= clear_pointer_tag |>
-       <| gprs_r9 ::= clear_pointer_tag |>
-       <| gprs_r10 ::= clear_pointer_tag |>
-       <| gprs_r11 ::= clear_pointer_tag |>
-       <| gprs_r12 ::= clear_pointer_tag |>
-       <| gprs_r13 ::= clear_pointer_tag |>
-       (* zero the rest *)
-       <| gprs_r14 := pv0 |>
-       <| gprs_r15 := pv0 |>
-     else
-       regs_state_zero <| gprs_r1 := PtrValue enc_ptr |>.
+  if is_system then
+    regs
+      <| gprs_r1 := PtrValue enc_ptr |>
+      <| gprs_r2 := far_call_r2      |>
+(* In system calls, preserve values in r3-r13 but clear ptr tags *)
+      <| gprs_r3 ::= clear_pointer_tag |>
+      <| gprs_r4 ::= clear_pointer_tag |>
+      <| gprs_r5 ::= clear_pointer_tag |>
+      <| gprs_r6 ::= clear_pointer_tag |>
+      <| gprs_r7 ::= clear_pointer_tag |>
+      <| gprs_r8 ::= clear_pointer_tag |>
+      <| gprs_r9 ::= clear_pointer_tag |>
+      <| gprs_r10 ::= clear_pointer_tag |>
+      <| gprs_r11 ::= clear_pointer_tag |>
+      <| gprs_r12 ::= clear_pointer_tag |>
+      <| gprs_r13 ::= clear_pointer_tag |>
+      (* zero the rest *)
+      <| gprs_r14 := pv0 |>
+      <| gprs_r15 := pv0 |>
+  else
+    regs_state_zero <| gprs_r1 := PtrValue enc_ptr |>.
 (*
 10. Form a new execution stack frame:
 
@@ -349,7 +349,7 @@ Definition regs_effect regs (is_system is_ctor:bool) ptr :=
    - it is a checkpoint that saves all storage states;
    - start PC at 0;
    - start SP at [INITIAL_SP_ON_FAR_CALL];
-*)
+ *)
 
 Definition CALL_IMPLICIT_PARAMETER_REG := R3.
 Inductive farcall_type : Set := Normal | Mimic | Delegate.
@@ -394,150 +394,158 @@ Definition select_ctx type (reg_ctx frame_ctx: u128) :=
   | Normal | Mimic => reg_ctx
   | Delegate => frame_ctx
   end.
-Definition new_code_shard_id (is_call_shard:bool) shard_provided caller_shard: shard_id :=
-  if is_call_shard
-  then shard_provided
-  else caller_shard.
 
-Definition new_this_shard_id type is_call_shard shard_provided caller_shard : shard_id :=
-  match type with
-  | Delegate => caller_shard
-  |_ => new_code_shard_id is_call_shard shard_provided caller_shard
-  end.
+Definition new_code_shard_id (is_call_shard:bool)
+  (provided current_shard:shard_id) : shard_id :=
+  if is_call_shard then provided else current_shard.
+
+Definition select_shards (type: farcall_type) (is_call_shard: bool) (provided: shard_id) (ss: shards) : shards :=
+  match ss with
+  | mk_shards old_this _ code =>
+      let new_caller := old_this in
+      let new_code := new_code_shard_id is_call_shard provided new_caller in
+      let new_this := match type with | Delegate => new_caller | _ => new_code end in
+      {|
+        shard_this := new_this;
+        shard_caller := new_caller;
+        shard_code := new_code;
+      |}       
+  end. 
 
 Section Def.
 
   Context (type:farcall_type) (dest_addr:contract_address) (handler_addr: code_address)
-    (call_as_static: bool) (shard_provided: bool) (abi_ptr_tag: bool).
+    (call_as_static: bool) (to_abi_shard: bool) (abi_ptr_tag: bool).
+
+  Context (xstack0: callstack).
   
-(* Not implemented yet: shards *)
-Inductive farcall : FarCall.params -> state -> state -> Prop :=
-| farcall_fwd_fatptr: forall flags old_regs old_pages xstack0 xstack1 xstack2 new_caller_stack gs reg_context_u128 new_pages new_code_page new_mem_ctx in_ptr to_shard ergs_query ergs_actual fwd_mode is_syscall_query out_ptr,
-    let old_extframe := topmost_extframe xstack0 in
-    let mem_ctx0 := old_extframe.(ecf_pages) in
-    let current_contract := old_extframe.(ecf_this_address) in
-    let is_system := addr_is_kernel dest_addr && is_syscall_query in
-    let allow_masking := negb is_system in
+  Let old_extframe := topmost_extframe xstack0.
+  Let mem_ctx0 := old_extframe.(ecf_pages).
+  Let current_contract := old_extframe.(ecf_this_address).
+  
+  (* Not implemented yet: shards *)
+  Inductive farcall : FarCall.params -> state -> state -> Prop :=
+  | farcall_fwd_fatptr: forall flags old_regs old_pages xstack0 xstack1 xstack2 new_caller_stack gs reg_context_u128 new_pages new_code_page new_mem_ctx in_ptr abi_shard ergs_query ergs_actual fwd_mode is_syscall_query out_ptr,
+      let is_system := addr_is_kernel dest_addr && is_syscall_query in
+      let allow_masking := negb is_system in
+      let callee_shard := if to_abi_shard then abi_shard else old_extframe.(ecf_shards).(shard_this) in
+      abi_ptr_tag = true ->
+      
+      paid_code_fetch allow_masking callee_shard gs.(gs_depot) gs.(gs_contracts) dest_addr xstack0 (xstack1, new_code_page) ->
+      paid_forward Ret.ForwardFatPointer (in_ptr, xstack1) (out_ptr, xstack2) ->
+      alloc_pages_extframe (old_pages,mem_ctx0) new_code_page (new_pages, new_mem_ctx) ->
+      pass_allowed_ergs (ergs_query,xstack2) (ergs_actual, new_caller_stack) ->
 
-    abi_ptr_tag = true ->
-    
-    paid_code_fetch allow_masking gs.(gs_depot) gs.(gs_contracts) dest_addr xstack0 (xstack1, new_code_page) ->
-    paid_forward Ret.ForwardFatPointer (in_ptr, xstack1) (out_ptr, xstack2) ->
-    alloc_pages_extframe (old_pages,mem_ctx0) new_code_page (new_pages, new_mem_ctx) ->
-    pass_allowed_ergs (ergs_query,xstack2) (ergs_actual, new_caller_stack) ->
+      let new_stack := ExternalCall {|
+                           ecf_this_address := select_this_address type current_contract dest_addr;
+                           ecf_msg_sender := select_sender type old_extframe.(ecf_msg_sender) current_contract old_regs;
+                           ecf_context_u128_value := select_ctx type reg_context_u128 old_extframe.(ecf_context_u128_value);
 
-    let new_stack := ExternalCall {|
-                         ecf_this_address := select_this_address type current_contract dest_addr;
-                         ecf_msg_sender := select_sender type old_extframe.(ecf_msg_sender) current_contract old_regs;
-                         ecf_context_u128_value := select_ctx type reg_context_u128 old_extframe.(ecf_context_u128_value);
+                           ecf_code_address := zero16;
+                           ecf_pages := new_mem_ctx;
+                           ecf_is_static :=  ecf_is_static old_extframe || call_as_static;
+                           ecf_saved_depot := gs.(gs_depot);
+                           ecf_shards := select_shards type to_abi_shard abi_shard old_extframe.(ecf_shards);
+                           ecf_common := {|
+                                          cf_exception_handler_location := handler_addr;
+                                          cf_sp := INITIAL_SP_ON_FAR_CALL;
+                                          cf_pc := zero16;
+                                          cf_ergs_remaining := ergs_actual;
+                                        |};
+                         |} (Some new_caller_stack) in
 
-                         ecf_code_address := zero16;
-                         ecf_pages := new_mem_ctx;
-                         ecf_is_static :=  ecf_is_static old_extframe || call_as_static;
-                         ecf_saved_depot := gs.(gs_depot);
-                         ecf_this_shard_id := new_this_shard_id type to_shard old_extframe.(ecf_this_shard_id);
-                         ecf_caller_shard_id := new_caller;
-                         ecf_code_shard_id := new_caller;
-                         ecf_common := {|
-                                        cf_exception_handler_location := handler_addr;
-                                        cf_sp := INITIAL_SP_ON_FAR_CALL;
-                                        cf_pc := zero16;
-                                        cf_ergs_remaining := ergs_actual;
-                                      |};
-                       |} (Some new_caller_stack) in
-
-    farcall
-            {|
-              memory_quasi_fat_ptr := in_ptr;
-              ergs_passed          := ergs_query;
-              FarCall.shard_id             := to_shard;
-              forwarding_mode      := fwd_mode;
-              constructor_call     := false;
-              to_system            := is_syscall_query;
-            |}
-            {|
-              gs_flags        := flags;
-              gs_regs         := old_regs;
-              gs_pages        := old_pages;
-              gs_callstack    := xstack0;
-              gs_context_u128 := reg_context_u128;
-
-
-              gs_global       := gs;
-            |}
-            {|
-              gs_flags        := flags_clear;
-              gs_regs         := regs_effect old_regs is_system false out_ptr;
-              gs_pages        := new_pages;
-              gs_callstack    := new_stack;
-              gs_context_u128 := zero128;
+      farcall
+        {|
+          memory_quasi_fat_ptr := in_ptr;
+          ergs_passed          := ergs_query;
+          FarCall.shard_id     := abi_shard;
+          forwarding_mode      := fwd_mode;
+          constructor_call     := false;
+          to_system            := is_syscall_query;
+        |}
+        {|
+          gs_flags        := flags;
+          gs_regs         := old_regs;
+          gs_pages        := old_pages;
+          gs_callstack    := xstack0;
+          gs_context_u128 := reg_context_u128;
 
 
-              gs_global       := gs;
-            |}
-| farcall_fwd_memory: forall gs flags old_regs old_pages xstack0 xstack1 xstack2 new_caller_stack reg_context_u128 new_pages new_code_page new_mem_ctx in_ptr to_shard ergs_query ergs_actual is_syscall_query out_ptr page_type,
-    let old_extframe := topmost_extframe xstack0 in
-    let current_contract := old_extframe.(ecf_this_address) in
-    let is_system := addr_is_kernel dest_addr && is_syscall_query in
-    let allow_masking := negb is_system in
-
-    paid_code_fetch allow_masking gs.(gs_depot) gs.(gs_contracts) dest_addr xstack0 (xstack1, new_code_page) ->
-    paid_forward (Ret.UseMemory page_type) (in_ptr, xstack1) (out_ptr, xstack2) ->
-    
-    let mem_ctx1 := (topmost_extframe xstack2).(ecf_pages) in
-    alloc_pages_extframe (old_pages, mem_ctx1) new_code_page (new_pages, new_mem_ctx) ->
-    pass_allowed_ergs (ergs_query,xstack2) (ergs_actual, new_caller_stack) ->
-
-    let new_stack := ExternalCall {|
-                         ecf_this_address := select_this_address type current_contract dest_addr;
-                         ecf_msg_sender := select_sender type old_extframe.(ecf_msg_sender) current_contract old_regs;
-                         ecf_context_u128_value := select_ctx type reg_context_u128 old_extframe.(ecf_context_u128_value);
-
-                         ecf_code_address := zero16;
-                         ecf_pages := new_mem_ctx;
-                         ecf_is_static :=  ecf_is_static old_extframe || call_as_static;
-                         ecf_saved_depot := gs.(gs_depot);
-                         ecf_common := {|
-                                        cf_exception_handler_location := handler_addr;
-                                        cf_sp := INITIAL_SP_ON_FAR_CALL;
-                                        cf_pc := zero16;
-                                        cf_ergs_remaining := ergs_actual;
-                                      |};
-                       |} (Some new_caller_stack) in
-
-    farcall 
-            {|
-              memory_quasi_fat_ptr := in_ptr;
-              ergs_passed          := ergs_query;
-              FarCall.shard_id             := to_shard;
-              forwarding_mode      := Ret.UseMemory page_type;
-              constructor_call     := false;
-              to_system            := is_syscall_query;
-            |}
-            {|
-              gs_flags        := flags;
-              gs_regs         := old_regs;
-              gs_pages        := old_pages;
-              gs_callstack    := xstack0;
-              gs_context_u128 := reg_context_u128;
+          gs_global       := gs;
+        |}
+        {|
+          gs_flags        := flags_clear;
+          gs_regs         := regs_effect old_regs is_system false out_ptr;
+          gs_pages        := new_pages;
+          gs_callstack    := new_stack;
+          gs_context_u128 := zero128;
 
 
-              gs_global       := gs;
-            |}
-            {|
-              gs_flags        := flags_clear;
-              gs_regs         := regs_effect old_regs is_system false out_ptr;
-              gs_pages        := new_pages;
-              gs_callstack    := new_stack;
-              gs_context_u128 := zero128;
+          gs_global       := gs;
+        |}
+  | farcall_fwd_memory: forall gs flags old_regs old_pages xstack0 xstack1 xstack2 new_caller_stack reg_context_u128 new_pages new_code_page new_mem_ctx in_ptr abi_shard ergs_query ergs_actual is_syscall_query out_ptr page_type,
+      let is_system := addr_is_kernel dest_addr && is_syscall_query in
+      let allow_masking := negb is_system in
+      let callee_shard := if to_abi_shard then abi_shard else old_extframe.(ecf_shards).(shard_this) in
 
-              gs_global       := gs;
-            |}
-.
+      paid_code_fetch allow_masking callee_shard gs.(gs_depot) gs.(gs_contracts) dest_addr xstack0 (xstack1, new_code_page) ->
+      paid_forward (Ret.UseMemory page_type) (in_ptr, xstack1) (out_ptr, xstack2) ->
+      
+      let mem_ctx1 := (topmost_extframe xstack2).(ecf_pages) in
+      alloc_pages_extframe (old_pages, mem_ctx1) new_code_page (new_pages, new_mem_ctx) ->
+      pass_allowed_ergs (ergs_query,xstack2) (ergs_actual, new_caller_stack) ->
+
+      let new_stack := ExternalCall {|
+                           ecf_this_address := select_this_address type current_contract dest_addr;
+                           ecf_msg_sender := select_sender type old_extframe.(ecf_msg_sender) current_contract old_regs;
+                           ecf_context_u128_value := select_ctx type reg_context_u128 old_extframe.(ecf_context_u128_value);
+
+                           ecf_shards := select_shards type to_abi_shard abi_shard old_extframe.(ecf_shards);
+                           ecf_code_address := zero16;
+                           ecf_pages := new_mem_ctx;
+                           ecf_is_static :=  ecf_is_static old_extframe || call_as_static;
+                           ecf_saved_depot := gs.(gs_depot);
+                           ecf_common := {|
+                                          cf_exception_handler_location := handler_addr;
+                                          cf_sp := INITIAL_SP_ON_FAR_CALL;
+                                          cf_pc := zero16;
+                                          cf_ergs_remaining := ergs_actual;
+                                        |};
+                         |} (Some new_caller_stack) in
+
+      farcall 
+        {|
+          memory_quasi_fat_ptr := in_ptr;
+          ergs_passed          := ergs_query;
+          FarCall.shard_id     := abi_shard;
+          forwarding_mode      := Ret.UseMemory page_type;
+          constructor_call     := false;
+          to_system            := is_syscall_query;
+        |}
+        {|
+          gs_flags        := flags;
+          gs_regs         := old_regs;
+          gs_pages        := old_pages;
+          gs_callstack    := xstack0;
+          gs_context_u128 := reg_context_u128;
+
+
+          gs_global       := gs;
+        |}
+        {|
+          gs_flags        := flags_clear;
+          gs_regs         := regs_effect old_regs is_system false out_ptr;
+          gs_pages        := new_pages;
+          gs_callstack    := new_stack;
+          gs_context_u128 := zero128;
+
+          gs_global       := gs;
+        |}
+  .
 End Def.
 
 Inductive fetch_operands abi dest handler:
-(contract_address * ExecutionStack.exception_handler * bool *  FarCall.params) -> Prop:=
+  (contract_address * exception_handler * bool *  FarCall.params) -> Prop:=
 
 | farcall_fetch: forall handler_location dest_val abi_val (abi_ptr_tag:bool) abi_params gs abi_ptr_tag,
     let fetch := resolve_fetch_value gs.(gs_regs) gs.(gs_callstack) gs.(gs_pages) in
@@ -553,25 +561,25 @@ Inductive fetch_operands abi dest handler:
     fetch_operands abi dest handler (dest_addr, handler_addr, abi_ptr_tag, abi_params).
 
 Inductive step : instruction -> smallstep :=
-                                        
+  
 | step_farcall_normal: forall (handler:imm_in) (abi dest:in_reg) call_shard call_as_static dest_addr handler_addr abi_ptr_tag abi_params gs gs',
 
     fetch_operands abi dest handler (dest_addr, handler_addr, abi_ptr_tag, abi_params)->
-    farcall Normal dest_addr handler_addr call_as_static abi_ptr_tag abi_params gs gs' ->
+    farcall Normal dest_addr handler_addr call_as_static abi_ptr_tag call_shard gs.(gs_callstack) abi_params gs gs' ->
 
     step (OpFarCall abi dest handler call_shard call_as_static) gs gs'
 
 | step_mimic: forall (handler:imm_in) (abi dest:in_reg) call_as_static dest_addr handler_addr abi_ptr_tag abi_params gs gs'
-  call_shard,
+                call_shard,
 
     fetch_operands abi dest handler (dest_addr, handler_addr, abi_ptr_tag, abi_params)->
-    farcall Mimic dest_addr handler_addr call_as_static abi_ptr_tag abi_params gs gs' ->
+    farcall Mimic dest_addr handler_addr call_as_static abi_ptr_tag call_shard gs.(gs_callstack) abi_params gs gs' ->
 
     step (OpMimicCall abi dest handler call_shard call_as_static) gs gs'
 | step_delegate: forall (handler:imm_in) (abi dest:in_reg) call_as_static dest_addr handler_addr abi_ptr_tag abi_params gs gs' call_shard,
 
     fetch_operands abi dest handler (dest_addr, handler_addr, abi_ptr_tag, abi_params)->
-    farcall Delegate dest_addr handler_addr call_as_static abi_ptr_tag abi_params gs gs' ->
+    farcall Delegate dest_addr handler_addr call_as_static abi_ptr_tag call_shard gs.(gs_callstack) abi_params gs gs' ->
 
     step (OpDelegateCall abi dest handler call_shard  call_as_static) gs gs'
 .
